Start working on `txn.Commit`

src/program_proof/mvcc/txn_commit.v
@@ -1,27 +1,138 @@
-From Perennial.program_proof.mvcc Require Import txn_common.
+From Perennial.program_proof.mvcc Require Import proph_proof txn_common txn_apply.
 
 Section program.
 Context `{!heapGS Σ, !mvcc_ghostG Σ}.
 
+(**
+ * Proof plan:
+ * 1. Prove FCC
+ * 2. Define [ptuple_past_rel]
+ * 3. Prove FCI
+ * 4. Prove CMT (incl. tuple-write safe extension)
+ * 5. Prove tuple-read safe extension
+ *)
+
 (* TODO: the last case also needs [¬ Q r w].*)
-Definition commit_false_cases γ : iProp Σ :=
-  (∃ tid, nca_tids_frag γ tid) ∨
-  (∃ tid, fa_tids_frag γ tid)  ∨
-  (∃ tmods, fci_tmods_frag γ tmods) ∨
-  (∃ tmods, fcc_tmods_frag γ tmods).
+Definition commit_false_cases tid γ : iProp Σ :=
+  (nca_tids_frag γ tid) ∨
+  (fa_tids_frag γ tid)  ∨
+  (∃ mods, fci_tmods_frag γ (tid, mods)) ∨
+  (∃ mods, fcc_tmods_frag γ (tid, mods)).
 
 Theorem wp_txn__Commit_false txn tid γ τ :
-  {{{ own_txn_ready txn tid γ τ ∗ commit_false_cases γ }}}
+  {{{ own_txn_ready txn tid γ τ ∗ commit_false_cases tid γ }}}
     Txn__Commit #txn
   {{{ (ok : bool), RET #ok; False }}}.
+Proof.
+  iIntros (Φ) "[Htxn Hfrag] HΦ".
+  wp_call.
+
+  (***********************************************************)
+  (* txn.apply()                                             *)
+  (***********************************************************)
+  wp_apply (wp_txn__apply with "Htxn").
+  iIntros "Htxn".
+  wp_pures.
+
+  (***********************************************************)
+  (* proph.ResolveCommit(txn.txnMgr.p, txn.tid, txn.wrbuf)   *)
+  (***********************************************************)
+  iNamed "Htxn".
+  iNamed "Himpl".
+  do 4 wp_loadField.
+  wp_apply (wp_ResolveCommit with "[$HwrbufRP]"); first eauto.
+  iInv "Hinv" as "> HinvO" "HinvC".
+  iApply ncfupd_mask_intro; first set_solver.
+  iIntros "Hclose".
+  iNamed "HinvO".
+  iExists future.
+  iFrame "Hproph".
+  iIntros "(%future' & %Hhead & Hproph)".
+
+  (* Obtain contradiction for each case. *)
+  unfold commit_false_cases.
+  iDestruct "Hfrag" as "[HncaFrag | Hfrag]".
+  { (* Case NCA. *)
+    iNamed "Hnca".
+    iDestruct (nca_tids_lookup with "HncaFrag HncaAuth") as "%Helem".
+    apply Hnca in Helem.
+    destruct (no_commit_abort_false Helem).
+    left.
+    set_solver.
+  }
+  iDestruct "Hfrag" as "[HfaFrag | Hfrag]".
+  { (* Case FA. *)
+    iNamed "Hfa".
+    iDestruct (fa_tids_lookup with "HfaFrag HfaAuth") as "%Helem".
+    apply Hfa in Helem.
+    destruct (first_abort_false mods Helem).
+    set_solver.
+  }
+  iDestruct "Hfrag" as "[HfciFrag | HfccFrag]".
+  { (* Case FCI. *)
+    iNamed "Hfci".
+    iDestruct "HfciFrag" as (m') "HfciFrag".
+    iDestruct (fci_tmods_lookup with "HfciFrag HfciAuth") as "%Helem".
+    apply Hfci in Helem. simpl in Helem.
+    (* TODO: Obtain contradiction by length of physical tuple. *)
+    admit.
+  }
+  { (* Case FCC. *)
+    iNamed "Hfcc".
+    iDestruct "HfccFrag" as (m') "HfccFrag".
+    iDestruct (fcc_tmods_lookup with "HfccFrag HfccAuth") as "%Helem".
+    apply Hfcc in Helem. simpl in Helem.
+    (* TODO: Obtain contradiction from [Q r w] and [¬ Q r w]. *)
+    admit.
+  }
 Admitted.
 
-Theorem wp_txn__Commit txn tid tmods γ τ :
-  {{{ own_txn_ready txn tid γ τ ∗ cmt_tmods_frag γ tmods }}}
+Theorem wp_txn__Commit txn tid mods γ τ :
+  {{{ own_txn_ready txn tid γ τ ∗ cmt_tmods_frag γ (tid, mods) }}}
     Txn__Commit #txn
   {{{ (ok : bool), RET #ok; own_txn_uninit txn γ }}}.
+Proof.
+  iIntros (Φ) "[Htxn Hfrag] HΦ".
+  wp_call.
+
+  (***********************************************************)
+  (* txn.apply()                                             *)
+  (***********************************************************)
+  wp_apply (wp_txn__apply with "Htxn").
+  iIntros "Htxn".
+  wp_pures.
+
+  (***********************************************************)
+  (* proph.ResolveCommit(txn.txnMgr.p, txn.tid, txn.wrbuf)   *)
+  (***********************************************************)
+  iNamed "Htxn".
+  iNamed "Himpl".
+  do 4 wp_loadField.
+  wp_apply (wp_ResolveCommit with "[$HwrbufRP]"); first eauto.
+  iInv "Hinv" as "> HinvO" "HinvC".
+  iApply ncfupd_mask_intro; first set_solver.
+  iIntros "Hclose".
+  iNamed "HinvO".
+  iExists future.
+  iFrame "Hproph".
+  iIntros "(%future' & %Hhead & Hproph)".
+
+  iNamed "Hcmt".
+  iDestruct (cmt_tmods_lookup with "Hfrag HcmtAuth") as "%Helem".
+  apply Hcmt in Helem. simpl in Helem.
+  (* TODO: Obtain equality between [mods] and [mods0] using [Helem] and [Hhead]. *)
+
+  (* TODO: Update the abstract part of the tuple RP to match the physical part. *)
+
+  (* TODO: Update the sets of ok/doomed txns to re-establish inv w.r.t. [future']. *)
+
+  (* TODO: Remove [(tid, mods)] from [tmods]. *)
+
+  (***********************************************************)
+  (* txn.txnMgr.deactivate(txn.sid, txn.tid)                 *)
+  (***********************************************************)
 Admitted.
 
 End program.
 
-Hint Extern 1 (environments.envs_entails _ (commit_false_cases _)) => unfold commit_false_cases : core.
+Hint Extern 1 (environments.envs_entails _ (commit_false_cases _ _)) => unfold commit_false_cases : core.
